Almost finished updates using finite maps

src/Semantics/AuxiliarDefinitions.v
@@ -13,75 +13,60 @@ Section Definitions.
 
   Variable CT : ClassTable.
   
-  Inductive fields : nat -> ClassName -> list Field -> Prop :=
-  | F_Obj : fields 0 Object nil
-  | F_Cls : forall C D CD fs fs' n,
+  Inductive fields : nat -> ClassName -> Map Field -> Prop :=
+  | F_Obj : fields 0 Object (M.empty _)
+  | F_Cls : forall C CD D fs fs' n,
       fs = cfields CD                                ->
-      In CD CT                                       ->
-      C = get_name CD                                ->
+      M.MapsTo C CD CT                               ->
+      D = cextends CD                                ->
       fields n D fs'                                 ->
-      NoDup (names (fs ++ fs'))                      -> 
-      fields (1 + n) C (fs ++ fs').
+      NoDup ((keys fs) ++ (keys fs'))                -> 
+      fields (1 + n) C (P.update fs fs').
     
   (* method type lookup *)
 
-  Reserved Notation "'mtype(' M ',' C ')' '=' Cs '~>' C1" (at level 40, Cs at next level).
-
-  Inductive m_type_lookup : Name -> ClassName -> list ClassName -> ClassName -> Prop :=
-  | mty_base : forall C C' D CD fs fsnodup K ms msnodup M MD args argsnodup body Cs,
-      In CD CT                                       ->
-      C = get_name CD                                ->
-      CD = mkClassDecl C D fs fsnodup K ms msnodup   ->
-      In MD ms                                       ->
-      M = get_name MD                                ->
-      MD = mkMethod C' M args argsnodup body         ->
+  Inductive m_type_lookup : nat -> Name -> ClassName -> list ClassName -> ClassName -> Prop :=
+  | mty_base : forall C C' CD ms M MD args Cs n,
+      M.MapsTo C CD CT                               ->
+      ms = cmethods CD                               ->
+      M.MapsTo M MD ms                               ->
+      args = margs MD                                ->
       Cs = map ftype args                            ->
-      mtype(M , C) = Cs ~> C'
-  | mty_step : forall C C' CD MD D fs fsnodup K ms M msnodup Cs,
-      In CD CT                                     ->
-      C = get_name CD                              ->
-      CD = mkClassDecl C D fs fsnodup K ms msnodup -> 
-      ~ In MD ms                                   ->
-      M = get_name MD                              ->
-      mtype(M, D) = Cs ~> C'                       ->
-      mtype(M, C) = Cs ~> C'
-  where "'mtype(' M ',' C ')' '=' Cs '~>' C1"
-          := (m_type_lookup M C Cs C1).
+      C' = mtype MD                                  ->
+      m_type_lookup n M C Cs C'
+  | mty_step : forall C C' CD D M Cs n,
+      M.MapsTo C CD CT                             ->
+      ~ M.In M (cmethods CD)                       ->
+      D = cextends CD                              ->
+      m_type_lookup n M D Cs C'                    ->
+      m_type_lookup (1 + n) M C Cs C'.
 
   (* method body lookup *)
 
-  Reserved Notation "'mbody(' m ',' D ')' '='  xs ';' e " (at level 40).
-
-  Inductive m_body_lookup : Name -> ClassName -> list ClassName -> Exp -> Prop :=
-  | mbody_base : forall C C' CD MD D fs fsnodup K ms msnodup M args argsnodup body ns,
-      CD = (mkClassDecl C D fs fsnodup K ms msnodup) ->
-      C  = get_name CD                               -> 
-      In CD CT                                       ->
-      M = get_name MD                                ->
-      MD = mkMethod C' M args argsnodup body         ->
-      In MD ms                                       ->
+  Inductive m_body_lookup : nat -> Name -> ClassName -> list ClassName -> Exp -> Prop :=
+  | mbody_base : forall C CD MD ms M args body ns n,
+      M.MapsTo C CD CT                               ->
+      ms = cmethods CD                               ->
+      M.MapsTo M MD ms                               ->
+      args = margs MD                                ->
       ns = map ftype args                            ->
-      mbody(M, C) =  ns ; body
-  | mbody_step : forall C CD MD D fs fsnodup K ms M msnodup ns body,
-      In CD CT                                      ->
-      CD = mkClassDecl C D fs fsnodup K ms msnodup  ->
-      C = get_name CD                               ->
-      ~ In MD ms                                    ->
-      M = get_name MD                               ->
-      mbody(M, D) =  ns ; body                      ->
-      mbody(M, C) =  ns ; body                    
-  where "'mbody(' M ',' D ')' '='  xs ';' e" := (m_body_lookup M D xs e).
+      body = mbody MD                                ->
+      m_body_lookup n M C ns body
+  | mbody_step : forall C CD D ms M ns body n,
+      M.MapsTo C CD CT                              ->
+      ms = cmethods CD                              ->
+      D = cextends CD                               ->
+      ~ M.In M ms                                   ->
+      m_body_lookup n M D ns body                   ->
+      m_body_lookup (1 + n) M C ns body.                    
 
   Hint Constructors m_body_lookup.
 
   (* valid method overriding *)
 
-  Reserved Notation "'override(' M ',' C ',' Cs ',' D ')'" (at level 40).
-
   Inductive valid_override : Name -> ClassName -> list ClassName -> ClassName -> Prop :=
-  | override_ok : forall  M C C0 Cs Ds D0,
-      mtype(M,C) = Ds ~> D0 -> Cs = Ds -> C0 = D0 -> override( M , C , Cs , C0)
-  where "'override(' M ',' C ',' Cs ',' D ')'" := (valid_override M C Cs D).
+  | override_ok : forall  M C C0 Cs Ds D0 n,
+      m_type_lookup n M C Ds D0 -> Cs = Ds -> C0 = D0 -> valid_override M C Cs C0.
 
   Hint Constructors valid_override.
 
@@ -115,14 +100,6 @@ End Definitions.
 
 Hint Constructors fields m_type_lookup m_body_lookup.
 
-Notation "mtype(' CT ',' M ',' C ')' '=' Cs '~>' C1" := (m_type_lookup CT M C Cs C1)
-                                                        (at level 40, Cs at level 60).
-
-Notation "'mbody(' CT ',' m ',' D ')' '='  xs ';' e " := (m_body_lookup CT m D xs e)(at level 40).
-
-Notation "'override(' CT ',' M ',' C ',' Cs ',' D ')'" := (valid_override CT M C Cs D)
-                                                            (at level 40).
-
 Notation " '[|' ds '\' xs '|]' e " := (substitution e ds xs) (at level 30).
 
 Section DEC.
@@ -130,17 +107,12 @@ Section DEC.
   Lemma fieldsDeterministic
      : forall n CT C fs, fields CT n C fs -> forall fs', fields CT n C fs' -> fs = fs'.
   Proof.
-    induction n ; intros.
-    +
-      inverts H ; inverts* H0.
-    +
-      inverts* H ; inverts* H0.
-      eapply IHn ; eauto.
-      eapply F_Cls.
+    induction n ; intros CT C fs H fs' H' ;
+      inverts H ; inverts* H' ; try map_solver ; fequals*.
   Qed.
   
   Definition fieldsDec : forall n CT C,
-    {fs | fields CT n C fs} + {forall fs, ~ fields CT n C fs}.
+      {fs | fields CT n C fs} + {forall fs, ~ fields CT n C fs}.
     refine (fix F n CT C : {fs | fields CT n C fs} +
                            {forall fs, ~ fields CT n C fs} :=
             match n as n'
@@ -148,33 +120,119 @@ Section DEC.
                                    {forall fs, ~ fields CT n C fs} with
             | 0    => fun _ =>
                match eq_nat_dec C Object with
-               | Yes => [|| nil ||]
+               | Yes => [|| (@M.empty Field)  ||]
                | No  => !!           
                end           
             | S n1 => fun _ =>
-               match find C CT with
-               | !! => !!
+               match MapsToDec C CT with
                | [|| CD ||] =>
-                 match find (cextends CD) CT with
+                 match F n1 CT (cextends CD) with
                  | !! => !!
-                 | [|| DD ||] =>
-                   match F n1 CT (cname DD) with
+                 | [|| fs' ||] =>
+                   match NoDup_dec eq_nat_dec ((keys (cfields CD)) ++ (keys fs')) with
+                   | Yes => [|| P.update (cfields CD) fs' ||]
+                   | No  => !!
+                   end           
+                 end  
+               | !!  => !!
+               end         
+            end (eq_refl n)) ; clear F ; simpl in * ; substs ; eauto ;
+             intros fs ; intro H ; inverts* H ; try map_solver.
+    +
+      apply (fieldsDeterministic _ _ _ _ f) in H4 ;  substs*.
+    +
+      apply n0 in H4 ; auto.
+  Defined.
+
+  Lemma m_type_lookupDeterministic :
+    forall CT n M C Cs C', m_type_lookup CT n M C Cs C' ->
+    forall Cs1 C1', m_type_lookup CT n M C Cs1 C1' -> Cs = Cs1 /\ C' = C1'.
+  Proof.
+    induction n ; intros M C Cs C' H Cs1 C1' H1 ;
+      inverts* H ; inverts* H1 ; try map_solver ; jauto.
+    eapply IHn ; eauto.
+  Qed.
+
+  Definition m_type_lookupDec
+    : forall n CT C M, {p | exists Cs C', m_type_lookup CT n M C Cs C' /\ p = (Cs , C')} +
+                       {forall Cs C', ~ m_type_lookup CT n M C Cs C'}.
+    refine (fix F n CT C M : {p | exists Cs C', m_type_lookup CT n M C Cs C' /\ p = (Cs , C')} +
+                             {forall Cs C', ~ m_type_lookup CT n M C Cs C'} :=
+              match n as n' return  n = n' ->
+                              {p | exists Cs C', m_type_lookup CT n M C Cs C' /\ p = (Cs , C')} +
+                              {forall Cs C', ~ m_type_lookup CT n M C Cs C'} with
+              | O => fun _ =>
+                 match MapsToDec C CT with
+                 | !! => !!
+                 | [|| CD ||] =>
+                   match MapsToDec M (cmethods CD) with
                    | !! => !!
-                   | [|| fs' ||] =>
-                     match NoDupDec eq_nat_dec (names (cfields CD ++ fs')) with
-                     | Yes => [|| cfields CD ++ fs' ||]
-                     | No  => !!           
-                     end
+                   | [|| MD ||] => [|| (map ftype (margs MD) , mtype MD) ||]
                    end
+                 end        
+              | S n1 => fun _ =>
+                 match MapsToDec C CT with
+                 | !! => !!
+                 | [|| CD ||] =>
+                   match MapsToDec M (cmethods CD) with
+                   | !! =>
+                     match F n1 CT (cextends CD) M with
+                     | !! => !!
+                     | [|| p ||] => [|| p ||]          
+                     end
+                   | [|| MD ||] => [|| (map ftype (margs MD) , mtype MD) ||]   
+                   end
+                 end          
+              end (eq_refl n)) ; clear F ; simpl in * ; substs* ;
+      try (intros ; intro H ; inverts* H) ; try map_solver.
+      apply n2 in H4 ; auto.
+  Defined.
+  
+  Lemma m_body_lookupDeterministic
+    : forall n CT M C Cs e,
+      m_body_lookup CT n M C Cs e ->
+      forall Cs1 e1,
+        m_body_lookup CT n M C Cs1 e1 ->
+        Cs = Cs1 /\ e = e1.
+  Proof.
+    induction n ; intros CT M C Cs e H Cs1 e1 H1
+    ; inverts* H ; inverts* H1 ; try map_solver ; jauto.
+    eapply IHn ; eauto.
+  Qed.
+
+  Definition m_body_lookupDec
+    : forall n CT M C, {p | exists Cs e, m_body_lookup CT n M C Cs e /\ p = (Cs , e)} +
+                       {forall Cs e, ~ m_body_lookup CT n M C Cs e}.
+    refine (fix F n CT M C : {p | exists Cs e, m_body_lookup CT n M C Cs e /\ p = (Cs , e)} +
+                             {forall Cs e, ~ m_body_lookup CT n M C Cs e} :=
+         match n as n'
+              return n = n' -> {p | exists Cs e, m_body_lookup CT n M C Cs e /\ p = (Cs , e)} +
+                               {forall Cs e, ~ m_body_lookup CT n M C Cs e} with
+         | 0 => fun _ =>
+             match MapsToDec C CT with
+             | !! => !!
+             | [|| CD ||] =>
+               match MapsToDec M (cmethods CD) with
+               | !! => !!
+               | [|| MD ||] => [|| (map ftype (margs MD) , mbody MD) ||]
+               end
+             end    
+         | S n1 => fun _ =>
+             match MapsToDec C CT with
+             | !! => !!
+             | [|| CD ||] =>
+               match MapsToDec M (cmethods CD) with
+               | !! =>
+                 match F n1 CT M (cextends CD) with
+                 | !! => !!
+                 | [|| p ||] => [|| p ||]          
                  end
-               end           
-            end (eq_refl n)) ; clear F ; simpl in * ; substs ;
-            try solve [intros ; intro H ; inverts* H] ; eauto ; intros ; try intro.
-    +
-      destruct* a.
-    +
-      destruct* a.
-      destruct* a0.
-      inverts* H.
-      
+               | [|| MD ||] => [|| (map ftype (margs MD) , mbody MD) ||]   
+               end
+             end                 
+         end (eq_refl n)) ; clear F ; simpl in * ; substs* ;
+      try (intros ; intro H ; inverts* H) ; try map_solver.
+      apply n2 in H5 ; auto.
+ Defined.   
 End DEC.
+
