src/Base/Environment.v
@@ -1,4 +1,5 @@
 Require Export
+        FJ.Base.Notations
 	OrderedTypeEx
         FMapAVL
         FMapFacts.
@@ -12,3 +13,19 @@ Module F := P.F.
 
 Definition Map := M.t.
 
+Definition keys {A : Type}(m : Map A) := M.fold (fun k _ ac => k :: ac) m nil.
+
+Definition values {A : Type}(m : Map A) := M.fold (fun _ v ac => v :: ac) m nil.
+
+Definition MapsToDec {A : Type}
+  : forall n (m : Map A), {C | M.MapsTo n C m} + {~ M.In n m}.
+  refine (fun n m =>
+            match M.find n m as r
+                  return M.find n m = r -> {C | M.MapsTo n C m} + {~ M.In n m} with
+            | None => fun _ => !!
+            | Some x => fun _ => [|| x ||]           
+            end (eq_refl (M.find n m))).
+  apply F.find_mapsto_iff ; auto.
+  intro H.
+  apply F.in_find_iff in H ; try contradiction.
+Defined.
